
# Exponential
An exponential function is a mathematical function of the form $a^x$
 where a is the constant and x is the variable. 
 
- For example if we see something like $a^x$ or $e^x$ 
- where `e` is Eulers Number which is 2.718

$$p(t)=p0​⋅a^t$$

- $p(t)$ represents the quantity of time
- `p0` represents the initial quantity when t is 0 
- `a` is the factor in which `p` changes for each unit increased by `t` 
- `t` is the time variable or variable 

$$p(t) =b\times a^t $$

- $p(t)$ is quantity of time t 
- `b` is another constant 
- `a` is the factor in with `p` changes per unit of `t`
- also in both cases a is the base number and `b` and `p0` is the initial value
- with `e` being the common base number in most exponential numbers 

The variable in a exponential is never constant its always changing this is specifically to `t` variable or the exponent variable

### Shifts 

$$
f(x) = a \cdot e^{b(x-h)} + k
$$

$$
f(x) = a \cdot e^{bx}
$$



## Notation 

- general form $f(x)=a^x$ of exponential's   

#growth rate this is related to the growth rate the base a and not being one displays the growth rate 



Considering the form for exponential's when we look at $0 < a < 1$ we are dealing with **exponential decay**

- since $a = 1/2$ when x =1 we have **$f(1) = 1/2$** which is less than 1 of course when we continue $f(2) = (1/2)^2 = 1/4$ x increasaes and $a^x$ gets smaller exponentially 

- $a > 1$ is for **exponential** since when we have $a =  2$ and get $x =1$ with$f(1) = 2$ as $x$ increases $f(x)$ grows rapidly therefore $a^x$ increases exponentially as $x$ increases. 

## Multiplying Exponential's with the same Base
If we have two exponential with the same base we must identify the usual form that it needs to be recognized in. like *lets say we multiply*  $a^n \times a^m$

   it would go as$$
f(x) = a^n \cdot a^m = a^{n+m}
$$

   - plug in random integers to give it a try it works

## Dividing Exponential with the Same  Base
Similarly when dividing exponential's with the same base we subtract the exponents 

$$
g(x) = \frac{a^n}{a^m} = a^{n-m}
$$


### Raising an Exponential to an Exponential

Now, if you have an exponential raised to another exponential:

$$
h(x) = (a^n)^m = a^{n \cdot m}
$$


### Combining it All

$$
p(x) = \frac{2^4 \cdot 3^2}{2^2} = 2^{4-2} \cdot 3^2 = 2^2 \cdot 9 = 36
$$

This is adding the said exponential's 


### Concavity 


![[240201_19h42m01s_screenshot.png]]

**half-life**: The half life of an exponential quantity is the time required for the quantity to be reduced by a factor of $1/2$ 

**double time**: for double is the increasing quantity time required for the quantity to double
